

Math notes

Memory growth factor of 2

Memory used with growth factor of 2

$$\begin{aligned}\sum_{i=0}^n 2^i &= 2^0 + 2^1 + 2^2 + 2^3 + \dots + 2^{n-1} + 2^n \\ &= 1 + 2 + 4 + 8 + \dots + 2^n\end{aligned}$$

Previous memory step:

$$\sum_{i=0}^{n-1} 2^i = 1 + 2 + 4 + 8 + \dots + 2^{n-1}$$

Let S be total history of memory freed

$$\begin{aligned}S &= 1 + 2 + 4 + 8 + \dots + 2^{n-1} \\ 2S &= 2 + 4 + 8 + 16 + \dots + 2^n\end{aligned}$$

To get S again:

$$\begin{aligned}S &= 2S - S \\ &= (2 + 4 + 8 + \dots + 2^{n-1} + 2^n) - (1 + 2 + 4 + 8 + \dots + 2^{n-1}) \\ &= 2^n - 1\end{aligned}$$

This will always be smaller than the new memory needed:

$$2^n + 1 < 2^n$$

Optimal growth factor

Let

- x be generalized growth factor
- n be realloc iteration

$$1, x, x^2, x^3, \dots, x^n$$

Summing series

Using formula for a geometric series $S_k = \frac{r^k - 1}{r - 1}$:

$$\frac{x^{n-1} - 1}{x - 1} \geq x^n$$

Determining equation for limit calc

Let R_n be ratio between reusable blocks and new block:

$$R_n = \frac{\sum_{i=0}^{n-2} x^i}{x^n}$$

If $R_n \geq 1$ we should be able to reuse previously freed memory.

$$\begin{aligned}
\lim_{n \rightarrow \infty} R_n &\geq 1 \\
\lim_{n \rightarrow \infty} \frac{\sum_{i=0}^{n-2} x^i}{x^n} &\geq 1 \\
\lim_{n \rightarrow \infty} \left(\frac{\frac{x^{n-1}-1}{x-1}}{x^n} \right) &\geq 1 \\
\lim_{n \rightarrow \infty} \left[\frac{x^{n-1}}{x^n(x-1)} - \frac{1}{x^n(x-1)} \right] &\geq 1
\end{aligned}$$

Quotient rule lets us subtract exponents of the same base:

$$\begin{aligned}
&\frac{x^{n-1}}{x^n} \\
&= x^{n-1-n} \\
&= x^{-1} \\
&= \frac{1}{x}
\end{aligned}$$

Thus

$$\begin{aligned}
\lim_{n \rightarrow \infty} \left[\frac{x^{n-1}}{x^n(x-1)} - \frac{1}{\frac{x^n}{x-1}} \right] &\geq 1 \\
\lim_{n \rightarrow \infty} \left[\frac{1}{x(x-1)} - \frac{1}{x^n(x-1)} \right] &\geq 1
\end{aligned}$$

Evaluating limit

$$\begin{aligned}
&\lim_{n \rightarrow \infty} \left[\frac{1}{x(x-1)} - \frac{1}{x^n(x-1)} \right] \\
&= \lim_{n \rightarrow \infty} \left[\frac{1}{x(x-1)} - 0 \right] \\
&= \frac{1}{x(x-1)}
\end{aligned}$$

Evaluating inequality

$$\begin{aligned}
\frac{1}{x(x-1)} &\geq 1 \\
1 &\geq x(x-1) \\
1 &\geq x^2 - x \\
0 &\geq x^2 - x - 1
\end{aligned}$$

Solving this quadratic equation yields:

$$\begin{aligned}
x_1 &= \frac{1 + \sqrt{5}}{2} \approx 1.618 \\
x_2 &= \frac{1 - \sqrt{5}}{2} \approx -0.618
\end{aligned}$$

the first of which is the golden ratio.

Compromise operation

$$n \times 1.5 = n + \left(\frac{n}{2}\right)$$

which is

$$n + (n \gg 1)$$

which should be pretty fast for a computer to do